platform/tests/ListBuilder.v
@@ -7,8 +7,8 @@ Import M.
 Module T := Thread0.Make(M).
 Import T.
 
-Definition handlerS := SPEC reserving 39
-  PREmain[_] sched * mallocHeap 0.
+Definition handlerS := SPEC reserving 49
+  Al fs, PREmain[_] sched fs * mallocHeap 0.
 
 Definition mainS := SPEC reserving 49
   PREmain[_] globalSched =?> 1 * mallocHeap 0.
@@ -21,10 +21,10 @@ Definition m := bimport [[ "malloc"!"malloc" @ [mallocS], "malloc"!"free" @ [fre
       "i" <- 0;; (* Loop counter *)
       "p" <- 0;; (* Pointer to head of list we will build *)
 
-      [PREmain[V] Ex ls, sll ls (V "p") * sched * mallocHeap 0]
+      [Al fs, PREmain[V] Ex ls, sll ls (V "p") * sched fs * mallocHeap 0]
       While ("i" < 10) {
         "r" <-- Call "malloc"!"malloc"(0, 2)
-        [PREmain[V, R] [| R <> 0 |] * [| freeable R 2 |] * R =?> 2 * Ex ls, sll ls (V "p") * sched * mallocHeap 0];;
+        [Al fs, PREmain[V, R] [| R <> 0 |] * [| freeable R 2 |] * R =?> 2 * Ex ls, sll ls (V "p") * sched fs * mallocHeap 0];;
 
         "r" *<- "i";;
         "r" + 4 *<- "p";;
@@ -32,32 +32,32 @@ Definition m := bimport [[ "malloc"!"malloc" @ [mallocS], "malloc"!"free" @ [fre
         "i" <- "i" + 1;;
 
         Yield
-        [PREmain[V] Ex ls, sll ls (V "p") * sched * mallocHeap 0]
+        [Al fs, PREmain[V] Ex ls, sll ls (V "p") * sched fs * mallocHeap 0]
       };;
 
-      [PREmain[V] Ex ls, sll ls (V "p") * sched * mallocHeap 0]
+      [Al fs, PREmain[V] Ex ls, sll ls (V "p") * sched fs * mallocHeap 0]
       While ("p" <> 0) {
         "r" <- "p";;
         "p" <-* "p" + 4;;
         Call "malloc"!"free"(0, "r", 2)
-        [PREmain[V] Ex ls, sll ls (V "p") * sched * mallocHeap 0];;
+        [Al fs, PREmain[V] Ex ls, sll ls (V "p") * sched fs * mallocHeap 0];;
 
         Yield
-        [PREmain[V] Ex ls, sll ls (V "p") * sched * mallocHeap 0]
+        [Al fs, PREmain[V] Ex ls, sll ls (V "p") * sched fs * mallocHeap 0]
       };;
 
-      Exit 40
+      Exit 50
     end with bfunctionNoRet "main"("x", "y") [mainS]
       Init
-      [PREmain[_] sched * mallocHeap 0];;
+      [Al fs, PREmain[_] sched fs * mallocHeap 0];;
 
-      Spawn("test"!"handler", 40)
-      [PREmain[_] sched * mallocHeap 0];;
+      Spawn("test"!"handler", 50)
+      [Al fs, PREmain[_] sched fs * mallocHeap 0];;
 
-      Spawn("test"!"handler", 40)
-      [PREmain[_] sched * mallocHeap 0];;
+      Spawn("test"!"handler", 50)
+      [Al fs, PREmain[_] sched fs * mallocHeap 0];;
 
-      Go 50
+      Exit 50
     end
   }}.
 
