platform/tests/ListBuilderAMD64.v
@@ -7,4 +7,4 @@ End M.
 Module E := Make(M).
 
 Set Printing Depth 999999.
-Eval compute in moduleS E.m5.
+Eval compute in moduleS E.m.
